Make the `list` stuff simpler since we don't really use `val_encode` anymore.

theories/utils/list.v
@@ -1,15 +1,13 @@
 From iris.heap_lang Require Export proofmode notation.
 From iris.heap_lang Require Import assert.
-From osiris.utils Require Export encodable.
 
 (** Immutable ML-style functional lists *)
-Instance list_val_enc `{ValEnc A} : ValEnc (list A) :=
-  fix go xs :=
-  let _ : ValEnc _ := @go in
-  match xs with
-  | [] => val_encode None
-  | x :: xs => val_encode (Some (x,xs))
-  end.
+Fixpoint llist (vs : list val) : val :=
+  match vs with
+  | [] => NONEV
+  | v :: vs => SOMEV (v,llist vs)
+  end%V.
+Arguments llist : simpl never.
 
 Definition lnil : val := λ: <>, NONEV.
 Definition lcons : val := λ: "x" "l", SOME ("x", "l").
@@ -48,15 +46,6 @@ Definition lreplicate : val :=
   rec: "go" "n" "x" :=
     if: "n" = #0 then lnil #() else
     let: "l" := "go" ("n" - #1) "x" in lcons "x" "l".
-
-Definition llist_member : val :=
-  rec: "go" "x" "l" :=
-    match: "l" with
-      NONE => #false
-    | SOME "p" =>
-      if: Fst "p" = "x" then #true
-      else let: "l" := (Snd "p")  in "go" "x" "l"
-    end.
 
 Definition llength : val :=
   rec: "go" "l" :=
@@ -97,195 +86,138 @@ Definition lsplit : val :=
   λ: "l", lsplit_at "l" ((llength "l") `quot` #2).
 
 Section lists.
-Context `{heapG Σ} `{ValEncDec A}.
+Context `{heapG Σ}.
 Implicit Types i : nat.
-Implicit Types x : A.
-Implicit Types xs : list A.
+Implicit Types v : val.
+Implicit Types vs : list val.
 
 Lemma lnil_spec :
-  {{{ True }}} lnil #() {{{ RET val_encode []; True }}}.
+  {{{ True }}} lnil #() {{{ RET llist []; True }}}.
 Proof. iIntros (Φ _) "HΦ". wp_lam. by iApply "HΦ". Qed.
 
-Lemma lcons_spec x xs :
-  {{{ True }}}
-    lcons (val_encode x) (val_encode xs)
-  {{{ RET val_encode (x :: xs); True }}}.
+Lemma lcons_spec v vs :
+  {{{ True }}} lcons v (llist vs) {{{ RET llist (v :: vs); True }}}.
 Proof. iIntros (Φ _) "HΦ". wp_lam. wp_pures. by iApply "HΦ". Qed.
 
-Lemma lisnil_spec xs:
+Lemma lisnil_spec vs:
   {{{ True }}}
-    lisnil (val_encode xs)
-  {{{ RET #(if xs is [] then true else false); True }}}.
-Proof. iIntros (Φ _) "HΦ". wp_lam. destruct xs; wp_pures; by iApply "HΦ". Qed.
+    lisnil (llist vs)
+  {{{ RET #(if vs is [] then true else false); True }}}.
+Proof. iIntros (Φ _) "HΦ". wp_lam. destruct vs; wp_pures; by iApply "HΦ". Qed.
 
-Lemma lhead_spec x xs:
-  {{{ True }}} lhead (val_encode (x::xs)) {{{ RET val_encode x; True }}}.
+Lemma lhead_spec v vs :
+  {{{ True }}} lhead (llist (v :: vs)) {{{ RET v; True }}}.
 Proof. iIntros (Φ _) "HΦ". wp_lam. wp_pures. by iApply "HΦ". Qed.
 
-Lemma ltail_spec x xs :
-  {{{ True }}} ltail (val_encode (x::xs)) {{{ RET val_encode xs; True }}}.
+Lemma ltail_spec v vs :
+  {{{ True }}} ltail (llist (v :: vs)) {{{ RET llist vs; True }}}.
 Proof. iIntros (Φ _) "HΦ". wp_lam. wp_pures. by iApply "HΦ". Qed.
 
-Lemma llookup_spec i xs x:
-  xs !! i = Some x →
-  {{{ True }}}
-    llookup #i (val_encode xs)
-  {{{ RET val_encode x; True }}}.
+Lemma llookup_spec i vs v :
+  vs !! i = Some v →
+  {{{ True }}} llookup #i (llist vs) {{{ RET v; True }}}.
 Proof.
-  iIntros (Hi Φ Hl) "HΦ".
-  iInduction xs as [|x' xs] "IH" forall (i Hi Hl);
+  iIntros (Hi Φ _) "HΦ".
+  iInduction vs as [|v' vs] "IH" forall (i Hi);
     destruct i as [|i]=> //; simplify_eq/=.
   { wp_lam. wp_pures. by iApply (lhead_spec with "[//]"). }
   wp_lam. wp_pures.
-  wp_apply (ltail_spec with "[//]"); iIntros (?). wp_let.
+  wp_apply (ltail_spec with "[//]"); iIntros (_). wp_let.
   wp_op. rewrite Nat2Z.inj_succ -Z.add_1_l Z.add_simpl_l. by iApply "IH".
 Qed.
 
-Lemma linsert_spec i xs x :
-  is_Some (xs !! i) →
-  {{{ True }}}
-    linsert #i (val_encode x) (val_encode xs)
-  {{{ RET val_encode (<[i:=x]>xs); True }}}.
+Lemma linsert_spec i vs v :
+  is_Some (vs !! i) →
+  {{{ True }}} linsert #i v (llist vs) {{{ RET llist (<[i:=v]>vs); True }}}.
 Proof.
-  iIntros ([w Hi] Φ Hl) "HΦ".
-  iInduction xs as [|x' xs] "IH" forall (i Hi Hl Φ);
+  iIntros ([w Hi] Φ _) "HΦ".
+  iInduction vs as [|v' vs] "IH" forall (i Hi Φ);
     destruct i as [|i]=> //; simplify_eq/=.
-  { wp_lam. wp_pures. wp_apply (ltail_spec with "[//]"). iIntros (?).
+  { wp_lam. wp_pures. wp_apply (ltail_spec with "[//]"); iIntros (_).
     wp_let. by iApply (lcons_spec with "[//]"). }
   wp_lam; wp_pures.
-  wp_apply (ltail_spec with "[//]"); iIntros (?). wp_let.
+  wp_apply (ltail_spec with "[//]"); iIntros (_). wp_let.
   wp_op. rewrite Nat2Z.inj_succ -Z.add_1_l Z.add_simpl_l.
-  wp_apply ("IH" with "[//] [//]"). iIntros (?). wp_let.
+  wp_apply ("IH" with "[//]"); iIntros (_).
   wp_apply (lhead_spec with "[//]"); iIntros "_".
   by wp_apply (lcons_spec with "[//]").
 Qed.
 
-(*
-Lemma llist_member_spec `{EqDecision A} (xs : list A) (x : A) :
-  {{{ True }}}
-    llist_member (val_encode x) (val_encode xs)
-  {{{ RET #(bool_decide (x ∈ xs)); True }}}.
-Proof.
-  iIntros (Φ Hl) "HΦ".
-  iInduction xs as [|x' xs] "IH" forall (Hl); simplify_eq/=.
-  { wp_lam; wp_pures. by iApply "HΦ". }
-  wp_lam; wp_pures.
-  destruct (bool_decide_reflect (val_encode x' = val_encode x)); simplify_eq/=; wp_if.
-  { rewrite (bool_decide_true (_ ∈ _ :: _)); last by left. by iApply "HΦ". }
-  wp_proj. wp_let. iApply ("IH" with "[//]").
-  destruct (bool_decide_reflect (x ∈ xs)).
-  - by rewrite bool_decide_true; last by right.
-  - by rewrite bool_decide_false ?elem_of_cons; last naive_solver.
-Qed.
-*)
-
-Lemma lreplicate_spec i x :
-  {{{ True }}}
-    lreplicate #i (val_encode x)
-  {{{ RET val_encode (replicate i x); True }}}.
+Lemma lreplicate_spec i v :
+  {{{ True }}} lreplicate #i v {{{ RET llist (replicate i v); True }}}.
 Proof.
   iIntros (Φ _) "HΦ". iInduction i as [|i] "IH" forall (Φ); simpl.
-  { wp_lam; wp_pures.
-    iApply (lnil_spec with "[//]"). iApply "HΦ". }
+  { wp_lam; wp_pures. iApply (lnil_spec with "[//]"); auto. }
   wp_lam; wp_pures.
   rewrite Nat2Z.inj_succ -Z.add_1_l Z.add_simpl_l.
-  wp_apply "IH"; iIntros (Hl). wp_let. by iApply (lcons_spec with "[//]").
+  wp_apply "IH"; iIntros (_). wp_let. by iApply (lcons_spec with "[//]").
 Qed.
 
-Lemma llength_spec xs :
-  {{{ True }}} llength (val_encode xs) {{{ RET #(length xs); True }}}.
+Lemma llength_spec vs :
+  {{{ True }}} llength (llist vs) {{{ RET #(length vs); True }}}.
 Proof.
-  iIntros (Φ Hl) "HΦ".
-  iInduction xs as [|x' xs] "IH" forall (Hl Φ); simplify_eq/=.
+  iIntros (Φ _) "HΦ".
+  iInduction vs as [|v' vs] "IH" forall (Φ); simplify_eq/=.
   { wp_lam. wp_match. by iApply "HΦ". }
   wp_lam. wp_match. wp_proj.
-  wp_apply ("IH" with "[//]"); iIntros "_ /=". wp_op.
+  wp_apply "IH"; iIntros "_ /=". wp_op.
   rewrite (Nat2Z.inj_add 1). by iApply "HΦ".
 Qed.
 
-Lemma lsnoc_spec xs x :
-  {{{ True }}}
-    lsnoc (val_encode xs) (val_encode x)
-  {{{ RET (val_encode (xs++[x])); True }}}.
+Lemma lsnoc_spec vs v :
+  {{{ True }}} lsnoc (llist vs) v {{{ RET (llist (vs ++ [v])); True }}}.
 Proof.
   iIntros (Φ _) "HΦ".
-  iInduction xs as [|x' xs] "IH" forall (Φ).
+  iInduction vs as [|v' vs] "IH" forall (Φ).
   { wp_rec. wp_pures. wp_lam. wp_pures. by iApply "HΦ". }
-  wp_rec.
-  wp_apply "IH"=> //.
-  iIntros (_). by wp_apply lcons_spec=> //.
+  wp_rec. wp_apply "IH"; iIntros (_). by wp_apply lcons_spec=> //.
 Qed.
 
-Lemma ltake_spec xs (n:Z) :
-  {{{ True }}}
-    ltake (val_encode xs) #n
-  {{{ RET val_encode (take (Z.to_nat n) xs); True }}}.
+Lemma ltake_spec vs (n : nat) :
+  {{{ True }}} ltake (llist vs) #n {{{ RET llist (take n vs); True }}}.
 Proof.
   iIntros (Φ _) "HΦ".
-  iInduction xs as [|x' xs] "IH" forall (n Φ).
-  - wp_rec. wp_pures. destruct (bool_decide (n ≤ 0)); wp_pures;
-      rewrite take_nil; by iApply "HΦ".
+  iInduction vs as [|x' vs] "IH" forall (n Φ).
   - wp_rec. wp_pures.
-    destruct (decide (n ≤ 0)).
-    + rewrite bool_decide_true=> //. wp_pures.
-      rewrite Z_to_nat_nonpos=> //.
-      rewrite firstn_O. by iApply "HΦ".
-    + rewrite bool_decide_false=> //.
-      wp_apply ("IH"); iIntros (_).
-      wp_apply (lcons_spec)=> //; iIntros (_).
-      rewrite -firstn_cons.
-      rewrite -Z2Nat.inj_succ; last lia.
-      rewrite Z.succ_pred.
-      by iApply "HΦ".
+    destruct (bool_decide (n ≤ 0)); wp_pures; rewrite take_nil; by iApply "HΦ".
+  - wp_rec; destruct n as [|n]; wp_pures; first by iApply "HΦ".
+    rewrite Nat2Z.inj_succ Z.sub_1_r Z.pred_succ.
+    wp_apply "IH"; iIntros (_).
+    wp_apply (lcons_spec with "[//]"); iIntros (_). by iApply "HΦ".
 Qed.
 
-Lemma ldrop_spec xs (n:Z) :
-  {{{ True }}}
-    ldrop (val_encode xs) #n
-  {{{ RET val_encode (drop (Z.to_nat n) xs); True }}}.
+Lemma ldrop_spec vs (n : nat) :
+  {{{ True }}} ldrop (llist vs) #n {{{ RET llist (drop n vs); True }}}.
 Proof.
   iIntros (Φ _) "HΦ".
-  iInduction xs as [|x' xs] "IH" forall (n Φ).
-  - wp_rec.
-    wp_pures. destruct (bool_decide (n ≤ 0)); wp_pures;
-      rewrite drop_nil; by iApply "HΦ".
+  iInduction vs as [|x' vs] "IH" forall (n Φ).
   - wp_rec. wp_pures.
-    destruct (decide (n ≤ 0)).
-    + rewrite bool_decide_true=> //. wp_pures.
-      rewrite Z_to_nat_nonpos=> //. rewrite drop_0.
-      by iApply "HΦ".
-    + rewrite bool_decide_false=> //.
-      wp_apply "IH"; iIntros (_).
-      rewrite -{1}(Z.succ_pred n) Z2Nat.inj_succ /= -Z.sub_1_r; last lia.
-      by iApply "HΦ".
+    destruct (bool_decide (n ≤ 0)); wp_pures; rewrite drop_nil; by iApply "HΦ".
+  - wp_rec; destruct n as [|n]; wp_pures; first by iApply "HΦ".
+    rewrite Nat2Z.inj_succ Z.sub_1_r Z.pred_succ.
+    wp_apply "IH"; iIntros (_). by iApply "HΦ".
 Qed.
 
-Lemma lsplit_at_spec xs n :
+Lemma lsplit_at_spec vs (n : nat) :
   {{{ True }}}
-    lsplit_at (val_encode (xs)) #n
-  {{{ RET val_encode (val_encode (take (Z.to_nat n) xs),
-          val_encode (drop (Z.to_nat n) xs)); True }}}.
+    lsplit_at (llist vs) #n
+  {{{ RET (llist (take n vs), llist (drop n vs)); True }}}.
 Proof.
-  iIntros (Φ _) "HΦ".
-  wp_lam.
-  wp_apply (ldrop_spec)=> //; iIntros (_).
-  wp_apply (ltake_spec)=> //; iIntros (_).
-  wp_pures.
-  by iApply "HΦ".
+  iIntros (Φ _) "HΦ". wp_lam.
+  wp_apply (ldrop_spec with "[//]"); iIntros (_).
+  wp_apply (ltake_spec with "[//]"); iIntros (_).
+  wp_pures. by iApply "HΦ".
 Qed.
 
-Lemma lsplit_spec xs :
+Lemma lsplit_spec vs :
   {{{ True }}}
-    lsplit (val_encode xs)
-  {{{ ys zs, RET (val_encode ys, val_encode zs); ⌜ ys++zs = xs ⌝ }}}.
+    lsplit (llist vs)
+  {{{ ws1 ws2, RET (llist ws1, llist ws2); ⌜ vs = ws1 ++ ws2 ⌝ }}}.
 Proof.
-  iIntros (Φ _) "HΦ".
-  wp_lam.
-  wp_apply (llength_spec)=>//; iIntros (_).
-  wp_apply (lsplit_at_spec)=>//; iIntros (_).
-  wp_pures.
-  iApply "HΦ".
-  iPureIntro.
-  apply take_drop.
+  iIntros (Φ _) "HΦ". wp_lam.
+  wp_apply (llength_spec with "[//]"); iIntros (_). wp_pures.
+  rewrite Z.quot_div_nonneg; [|lia..]. rewrite -(Z2Nat_inj_div _ 2).
+  wp_apply (lsplit_at_spec with "[//]"); iIntros (_).
+  iApply "HΦ". by rewrite take_drop.
 Qed.
 End lists.
