theories/examples/sort_client.v
@@ -7,27 +7,21 @@ From osiris.examples Require Import sort.
 Section sort_client.
   Context `{!heapG Σ, !proto_chanG Σ} (N : namespace).
 
-  Local Arguments val_encode _ _ !_ /.
-
   Lemma sort_client_le_spec l (xs : list Z) :
-    {{{ l ↦ val_encode xs }}}
+    {{{ l ↦ llist (LitV ∘ LitInt <$> xs) }}}
       sort_client cmpZ #l
-    {{{ ys, RET #(); ⌜Sorted (≤) ys⌝ ∗ ⌜ ys ≡ₚ xs⌝ ∗ l ↦ val_encode ys }}}.
+    {{{ ys, RET #(); ⌜Sorted (≤) ys⌝ ∗ ⌜ ys ≡ₚ xs⌝ ∗ l ↦ llist (LitV ∘ LitInt <$> ys) }}}.
   Proof.
-    assert (∀ zs : list Z, val_encode zs = val_encode (LitV ∘ LitInt <$> zs)) as Henc.
-    { intros zs. induction zs; f_equal/=; auto with f_equal. }
     iIntros (Φ) "Hl HΦ".
     iApply (sort_client_spec N IZ (≤) _ _ (LitV ∘ LitInt <$> xs) xs with "[] [Hl] [HΦ]").
     { iApply cmpZ_spec. }
-    { rewrite -Henc. iFrame "Hl".
-      iInduction xs as [|x xs] "IH"; csimpl; first by iFrame.
-      by iFrame "IH". }
+    { iFrame "Hl". iInduction xs as [|x xs] "IH"; csimpl; by iFrame "#". }
     iIntros "!>" (ys ws) "(?&?&?&HI)".
     iAssert ⌜ ws = (LitV ∘ LitInt) <$> ys ⌝%I with "[HI]" as %->.
     { iInduction ys as [|y ys] "IH" forall (ws);
-      destruct ws as [|w ws]; csimpl; try done.
+        destruct ws as [|w ws]; csimpl; try done.
       iDestruct "HI" as "[-> HI2]".
       by iDestruct ("IH" with "HI2") as %->. }
-    rewrite -Henc. iApply ("HΦ" $! ys with "[$]").
+    iApply ("HΦ" $! ys with "[$]").
   Qed.
 End sort_client.
